x86/RawAsmgen.v
@@ -4,6 +4,7 @@ Require Import Asm.
 Require Import Integers.
 Require Import List.
 Require Import ZArith.
+Require Memimpl.
 Require Import Memtype.
 Require Import Memory.
 Require Import Archi.
@@ -16,7 +17,13 @@ Require Import Conventions1.
 
 Section WITHMEMORYMODEL.
 
-  Context `{memory_model_ops: Mem.MemoryModelOps}.
+  Class MemoryModelSingleStack {mem} `{memory_model: Mem.MemoryModel mem} :=
+    {
+      size_stack_below:
+        forall m: mem, Memimpl.Mem.size_stack (Memtype.Mem.stack_adt m) < Memimpl.Mem.stack_limit;
+    }.
+  
+  Context `{memory_model: MemoryModelSingleStack}.
 
   Existing Instance mem_accessors_default.
 
@@ -25,7 +32,7 @@ Section WITHMEMORYMODEL.
   Definition exec_instr {F V} (ge: Genv.t F V) f i rs m :=
     match i with
     | Pallocframe fi ofs_ra ofs_link =>
-      let sp := Val.offset_ptr (rs # RSP) (Ptrofs.repr (- (frame_size fi))) in
+      let sp := Val.offset_ptr (rs # RSP) (Ptrofs.repr (- align (Z.max 0 (frame_size fi)) 8)) in
       match Mem.storev Mptr m (Val.offset_ptr sp ofs_link) rs#RSP with
       | None => Stuck
       | Some m2 =>
@@ -40,11 +47,7 @@ Section WITHMEMORYMODEL.
       | Some ra =>
         match Mem.loadv Mptr m (Val.offset_ptr rs#RSP ofs_link) with
         | None => Stuck
-        | Some sp =>
-          match rs#RSP with
-          | Vptr stk ofs => Next (nextinstr (rs#RSP <- sp #RA <- ra)) m
-          | _ => Stuck
-          end
+        | Some sp => Next (nextinstr (rs#RSP <- sp #RA <- ra)) m
         end
       end
     | _ => Asm.exec_instr ge f i rs m
@@ -86,25 +89,206 @@ Section WITHMEMORYMODEL.
   Variable prog: Asm.program.
   Let ge := Genv.globalenv prog.
 
-  Inductive match_states: state -> state -> Prop := 
+  Variable bstack: block.
+  Variable id_stack: ident.
+  Hypothesis find_bstack: Genv.find_symbol ge id_stack = Some bstack. 
+  Hypothesis repr_stack_limit:
+    Memimpl.Mem.stack_limit < Ptrofs.max_unsigned.
+
+
+
+  Lemma size_stack_pos:
+    forall l,
+      0 <= Memimpl.Mem.size_stack l.
+  Proof.
+    induction l; simpl; intros; eauto. omega.
+    destruct a.
+    generalize (align_le (Z.max 0 z) 8) (Z.le_max_l 0 z); omega.
+  Qed.
+  
+  Definition no_inject_below j m thr:=
+    forall b delta o k p,
+      j b = Some (bstack, delta) ->
+      Mem.perm m b o k p ->
+      thr <= o + delta.
+
+  Definition agree_sp m1 rs2:=
+    forall ostack,
+      rs2 # RSP = Vptr bstack ostack ->
+      Ptrofs.unsigned ostack = Memimpl.Mem.stack_limit - Memimpl.Mem.size_stack (Mem.stack_adt m1).
+
+  Definition perm_bstack m2:=
+    forall (ofs : Z) (k : perm_kind) (p : permission),
+       Mem.perm m2 bstack ofs k p -> 0 <= ofs < Ptrofs.max_unsigned.
+
+  Definition perm_bstack_stack_limit m2:=
+    forall (ofs : Z) (k : perm_kind) (p : permission),
+      0 <= ofs < Memimpl.Mem.stack_limit ->
+      Mem.perm m2 bstack ofs k p.
+
+  Definition sp_aligned rs2:=
+    forall ostack,
+      rs2 # RSP = Vptr bstack ostack ->
+      (8 | Ptrofs.unsigned ostack).
+
+  Definition no_stack m2 :=
+    Mem.stack_adt m2 = nil.
+  
+
+  
+
+  
+  Lemma alloc_inject:
+    forall j m1 m2 (rs1 rs2: regset) fi m' b m1',
+      Mem.inject j m1 m2 ->
+      Mem.valid_block m2 bstack ->
+      (forall r, Val.inject j (rs1#r) (rs2#r)) ->
+      Mem.alloc m1 0 (frame_size fi) = (m', b) ->
+      Mem.record_stack_blocks m' (inl (b, Some fi)) (frame_size fi) = Some m1' ->
+      agree_sp m1 rs2 ->
+      sp_aligned rs2 ->
+      perm_bstack m2 ->
+      perm_bstack_stack_limit m2 ->
+      no_stack m2 ->
+      forall ostack,
+        rs2 # RSP = Vptr bstack ostack ->
+        no_inject_below j m1 (Ptrofs.unsigned ostack) ->
+      let newostack := Ptrofs.unsigned ostack - align (Z.max 0 (frame_size fi)) 8 in
+      let rs2' := (rs2 # RSP <- (Vptr bstack (Ptrofs.repr newostack))) in
+      exists j',
+        (forall bb, j' bb = if peq bb b then Some (bstack, newostack) else j bb) 
+        /\ inject_incr j j'
+      /\ no_inject_below j' m1' newostack
+      /\ Mem.inject j' m1' m2
+      /\ agree_sp m1' rs2'
+      /\ sp_aligned rs2'.
+  Proof.
+    intros j m1 m2 rs1 rs2 fi m' b m1' MINJ VB RINJ ALLOC RSB AGSP SPAL PBS PBSL NOSTACK ostack EQRSP NIB.
+    set (newostack := Ptrofs.unsigned ostack - align (Z.max 0 (frame_size fi)) 8).
+    simpl; intros.
+    assert (REPR: 0 <= newostack < Ptrofs.max_unsigned).
+    {
+      unfold newostack.
+      generalize (size_stack_below m1').
+      erewrite Mem.record_stack_block_stack_adt. 2: eauto.
+      simpl.
+      erewrite Mem.alloc_stack_blocks. 2: eauto.
+      erewrite AGSP; eauto.
+      split.  omega.
+      generalize (size_stack_pos (Mem.stack_adt m1)); intros.
+      generalize (align_le (Z.max 0 (frame_size fi)) 8) (Z.le_max_l 0 (frame_size fi)).
+      omega.
+    }
+    generalize (Mem.alloc_left_mapped_inject _ _ _ _ _ _ _ _ newostack MINJ ALLOC VB).
+    intro A.
+    trim A.
+    {
+      omega.
+    }
+    trim A.
+    {
+      intros; right; eapply PBS; eauto.
+    }
+    trim A.
+    {
+      intros; eapply PBSL; eauto.
+      unfold newostack. rewrite AGSP; auto.
+      generalize (size_stack_below m1').
+      erewrite Mem.record_stack_block_stack_adt. 2: eauto.
+      simpl.
+      erewrite Mem.alloc_stack_blocks. 2: eauto.
+      split.  omega.
+      cut (ofs < Memimpl.Mem.size_stack (Mem.stack_adt m1) + align (Z.max 0 (frame_size fi)) 8). omega.
+      eapply Z.lt_le_trans. apply H.
+      generalize (size_stack_pos (Mem.stack_adt m1)); intros.
+      generalize (align_le (Z.max 0 (frame_size fi)) 8) (Z.le_max_l 0 (frame_size fi)).
+      rewrite Z.max_r by omega.
+      omega. 
+    }
+    trim A.
+    {
+      red.
+      intros.
+      unfold newostack.
+      eapply Zdivides_trans with 8.
+      destruct chunk; try (exists 8; reflexivity);
+        try (exists 4; reflexivity);
+        try (exists 2; reflexivity);
+        try (exists 1; reflexivity).
+      apply Z.divide_sub_r.
+      apply SPAL; auto.
+      apply align_divides. omega.
+    }
+    trim A.
+    {
+      intros b0 delta' ofs k p JB PERM RNG.
+      generalize (NIB _ _ _ _ _ JB PERM).
+      unfold newostack in RNG.
+      rewrite Z.max_r in RNG by omega. simpl in RNG.
+      generalize (align_le (frame_size fi) 8).
+      omega.
+    }
+    trim A.
+    {
+      rewrite NOSTACK. simpl. easy.
+    }
+    destruct A as (f' & MINJ' & INCR & EQ1 & EQ2).
+    exists f'.
+    split; [|split; [|split; [|split;[|split]]]].
+    - intros. destruct peq; subst; auto.
+    - red; intros.
+      destruct (peq b0 b); auto.
+    - red. intros b0 delta o k p JB PERM.
+      eapply Mem.record_stack_block_perm in PERM.
+      eapply Mem.perm_alloc_inv in PERM; eauto. 
+      destruct peq.
+      + subst. rewrite EQ1 in JB. inv JB. omega.
+      + transitivity (Ptrofs.unsigned ostack).
+        generalize (Z.le_max_l 0 (frame_size fi)); intro MAX.
+        generalize (align_le (Z.max 0 (frame_size fi)) 8). unfold newostack. omega.
+        eapply NIB; eauto. erewrite <- EQ2; eauto.
+      + eauto.
+    - admit.
+    - red. rewrite Pregmap.gss. inversion 1. subst.
+      erewrite Mem.record_stack_block_stack_adt. 2: eauto.
+      simpl. erewrite Mem.alloc_stack_blocks. 2: eauto.
+      rewrite Ptrofs.unsigned_repr.
+      unfold newostack in *. rewrite (AGSP _ EQRSP).
+      omega. omega.
+    - red; intros. rewrite Pregmap.gss in H. inversion H. subst.
+      rewrite Ptrofs.unsigned_repr by omega.
+      unfold newostack.
+      apply Z.divide_sub_r.
+      apply SPAL; auto.
+      apply align_divides. omega.
+  Admitted.
+  
+  Inductive match_states: meminj -> state -> state -> Prop := 
   | match_states_intro:
-      forall j rs m rs' m' bnd
+      forall j (rs: regset) m (rs': regset) m' bnd
         (MINJ: Mem.inject j m m')
         (RINJ: forall r, Val.inject j (rs # r) (rs' # r))
+        (VB: Mem.valid_block m' bstack)
+        (AGSP: agree_sp m rs')
+        (SPAL: sp_aligned rs')
+        (PBS: perm_bstack m')
+        (PBSL: perm_bstack_stack_limit m')
+        (NS: no_stack m')
+        ostack
+        (RSPEQ: rs' RSP = Vptr bstack ostack)
+        (NIB: no_inject_below j m (Ptrofs.unsigned ostack))
         (MPG: Separation.globalenv_preserved ge j bnd)
       ,
-        match_states (State rs m) (State rs' m').
+        match_states j (State rs m) (State rs' m').
 
   Axiom exec_instr_inject:
     forall j m1 m2 rs1 rs2 f i rs1' m1',
-      Mem.inject j m1 m2 ->
-      (forall r, Val.inject j (rs1#r) (rs2#r)) ->
+      match_states j (State rs1 m1) (State rs2 m2) ->
       Asm.exec_instr ge f i rs1 m1 = Next rs1' m1' ->
       exists j' rs2' m2',
         Asm.exec_instr ge f i rs2 m2 = Next rs2' m2'
-        /\ Mem.inject j' m1' m2'
-        /\ (forall r, Val.inject j' (rs1'#r) (rs2'#r))
-        /\ inject_incr j j'.
+        /\ match_states j' (State rs1' m1') (State rs2' m2')
+        /\ inject_incr j j'. 
   (* should be proved already somewhere *)
 
   Definition is_unchanged (i: instruction) :=
@@ -114,38 +298,32 @@ Section WITHMEMORYMODEL.
     | _ => true
     end.
 
-  Variable bstack: block.
-  Variable id_stack: ident.
-  Hypothesis find_bstack: Genv.find_symbol ge id_stack = Some bstack. 
-
-  Lemma alloc_inject:
-    forall j m1 m2 rs1 rs2 f i rs1' m1',
-      Mem.inject j m1 m2 ->
-      (forall r, Val.inject j (rs1#r) (rs2#r)) ->
-      Mem.alloc m 0 (frame_size fi) = (m', b) ->
-      Mem.record_stack_blocks m' (inl (b, Some fi)) (frame_size fi) = Some m'' ->
-      rs2 # RSP = 
-      exists j',
-        j' b = 
-
   Lemma exec_instr_inject':
     forall j m1 m2 rs1 rs2 f i rs1' m1',
-      Mem.inject j m1 m2 ->
-      (forall r, Val.inject j (rs1#r) (rs2#r)) ->
+      match_states j (State rs1 m1) (State rs2 m2) ->
       Asm.exec_instr ge f i rs1 m1 = Next rs1' m1' ->
       exists j' rs2' m2',
         exec_instr ge f i rs2 m2 = Next rs2' m2'
-        /\ Mem.inject j' m1' m2'
-        /\ (forall r, Val.inject j' (rs1'#r) (rs2'#r))
+        /\ match_states j' (State rs1' m1') (State rs2' m2')
         /\ inject_incr j j'.
   Proof.
-    intros. destruct (is_unchanged i) eqn:?.
-    edestruct exec_instr_inject; eauto.
-    destruct i; simpl in *; eauto; try congruence.
-    destruct i; simpl in *; try congruence.
-    -                           (* allocframe *)
-      repeat destr_in H1.
-      
+    intros.
+    destruct (is_unchanged i) eqn:?.
+    - edestruct exec_instr_inject; eauto.
+      destruct i; simpl in *; eauto; try congruence.
+    - destruct i; simpl in *; try congruence.
+      + (* allocframe *)
+        repeat destr_in H0. inv H.
+        edestruct alloc_inject as (j' & JSPEC & INCR & NIB' & MINJ' & AGSP' & SPAL') ; eauto.
+        rewrite RSPEQ.  simpl.
+        exploit Mem.store_mapped_inject. apply MINJ'. eauto. rewrite JSPEC. rewrite pred_dec_true. eauto. auto.
+        eapply val_inject_incr; eauto. intros (n2 & STORE & MINJ2).
+        rewrite Ptrofs.add_zero_l in STORE.
+        unfold Ptrofs.add.
+        rewrite Mem.address_inject.
+        
+
+        rewrite STORE.
   Qed.
 
   
